src/Examples/AtomicPair/AtomicPairAPI.v
@@ -35,5 +35,6 @@ Module AtomicPair.
        crash_total := crash_total_ok;
        finish_total := crash_total_ok;
        crash_non_err := crash_non_err_ok;
+       finish_non_err := crash_non_err_ok;
        initP := fun s => s = (0, 0) |}.
 End AtomicPair.
