src/Examples/StatDb/Impl.v
@@ -38,6 +38,7 @@ Module DB.
        crash_total := crash_total_ok;
        finish_total := crash_total_ok;
        crash_non_err := crash_non_err_ok;
+       finish_non_err := crash_non_err_ok;
        initP := fun s => s = nil |}.
 End DB.
 
